Lowering (WIP).

DeBruijn.v
@@ -141,14 +141,14 @@ Instance Lift_idx : Lift nat := {
     if le_gt_dec k x then w + x else x
 }.
 
-(* Unlift? *)
-Class Unlift (T : Type) := {
-  unlift:
+(* Lowering, the inverse operation to lifting *)
+Class Lower (T : Type) := {
+  lower:
     nat -> nat -> T -> T
 }.
 
-Instance Unlift_idx : Unlift nat := {
-  unlift w k x :=
+Instance Lower_idx : Lower nat := {
+  lower w k x :=
     if le_gt_dec k x then x - w else x
 }.
 
@@ -165,8 +165,10 @@ Instance Unlift_idx : Unlift nat := {
 
 Notation shift :=
   (lift 1).
-Notation unshift :=
-  (unlift 1).
+
+(* [drop k t] is an abbreviation for [lower 1 k t] *)
+Notation drop :=
+  (lower 1).
 
 (* [subst v k t] is the term obtained by substituting the value [v] for
    the variable [k] in the term [t]. *)
@@ -645,17 +647,17 @@ Proof.
   reflexivity.
 Qed.
 
-(* Generic definition of [unlift] in terms of [traverse]. *)
-Instance Unlift_Traverse `{Var V, Traverse V T} : Unlift T := {
-  unlift w k t :=
-    traverse (fun l x => var (unlift w (l + k) x)) 0 t
+(* Generic definition of [lower] in terms of [traverse]. *)
+Instance Lower_Traverse `{Var V, Traverse V T} : Lower T := {
+  lower w k t :=
+    traverse (fun l x => var (lower w (l + k) x)) 0 t
 }.
 
-Lemma expand_unlift:
+Lemma expand_lower:
   forall `{Var V, Traverse V T},
   forall w k t,
-  unlift w k t =
-  traverse (fun l x => var (unlift w (l + k) x)) 0 t.
+  lower w k t =
+  traverse (fun l x => var (lower w (l + k) x)) 0 t.
 Proof.
   reflexivity.
 Qed.
@@ -693,14 +695,14 @@ Proof.
   just_do_it.
 Qed.
 
-Lemma recognize_unlift:
+Lemma recognize_lower:
   forall `{Var V, Traverse V T},
   TraverseRelative ->
   forall w k1 k2 t,
   forall traverse_,
   traverse_ = traverse -> (* helps rewrite *)
-  traverse_ (fun l x => var (unlift w (l + k2) x)) k1 t =
-  unlift w (k1 + k2) t.
+  traverse_ (fun l x => var (lower w (l + k2) x)) k1 t =
+  lower w (k1 + k2) t.
 Proof.
   intros. subst. simpl.
   eapply traverse_relative; [ | instantiate (1 := k1); omega ].
@@ -714,8 +716,8 @@ Ltac recognize_lift :=
   rewrite recognize_lift by eauto with typeclass_instances;
   repeat rewrite plus_0_l. (* useful when [k1] is zero *)
 
-Ltac recognize_unlift :=
-  rewrite recognize_unlift by eauto with typeclass_instances;
+Ltac recognize_lower :=
+  rewrite recognize_lower by eauto with typeclass_instances;
   repeat rewrite plus_0_l. (* useful when [k1] is zero *)
 
 Ltac recognize_lift_in h :=
@@ -775,12 +777,12 @@ Ltac simpl_lift :=
   
   end.
 
-Ltac simpl_unlift :=
+Ltac simpl_lower :=
   match goal with
 
   (* Case: [_traverse] appears in the goal. *)
   (* this binds the meta-variable [_traverse] to the user's [traverse_term] *)
-  |- context[?_traverse (fun l x : nat => var (unlift ?w (l + ?k) x)) _ _] =>
+  |- context[?_traverse (fun l x : nat => var (lower ?w (l + ?k) x)) _ _] =>
       (* this causes the reduction of the fixpoint: *)
     unfold _traverse; fold _traverse;
     (* we now have a term of the form [TApp (traverse_term ...) ...].
@@ -789,13 +791,13 @@ Ltac simpl_unlift :=
     (* use [recognize_lift] at the specific type of the [_traverse] function
        that we have just simplified *)
     match type of _traverse with (nat -> nat -> ?V) -> nat -> ?T -> ?T =>
-      repeat rewrite (@recognize_unlift V _ T _ _) by eauto with typeclass_instances
+      repeat rewrite (@recognize_lower V _ T _ _) by eauto with typeclass_instances
     end;
     repeat rewrite plus_0_l (* useful when [k1] is zero and we are at a leaf *)
 
   (* Case: [_traverse] appears in a hypothesis. *)
   (* this binds the meta-variable [_traverse] to the user's [traverse_term] *)
-  | h: context[?_traverse (fun l x : nat => var (unlift ?w (l + ?k) x)) _ _] |- _ =>
+  | h: context[?_traverse (fun l x : nat => var (lower ?w (l + ?k) x)) _ _] |- _ =>
     (* this causes the reduction of the fixpoint: *)
     unfold _traverse in h; fold _traverse in h;
     (* we now have a term of the form [TApp (traverse_term ...) ...].
@@ -804,7 +806,7 @@ Ltac simpl_unlift :=
     (* use [recognize_lift] at the specific type of the [_traverse] function
        that we have just simplified *)
     match type of _traverse with (nat -> nat -> ?V) -> nat -> ?T -> ?T =>
-      repeat rewrite (@recognize_unlift V _ T _ _)  in h by eauto with typeclass_instances
+      repeat rewrite (@recognize_lower V _ T _ _)  in h by eauto with typeclass_instances
     end;
     repeat rewrite plus_0_l in h (* useful when [k1] is zero and we are at a leaf *)
   
@@ -824,15 +826,15 @@ Ltac simpl_lift_goal :=
   (* if this exposes uses of [var], replace them with the user's [TVar] constructor *)
   simpl var.
 
-Ltac simpl_unlift_goal :=
+Ltac simpl_lower_goal :=
   (* this replaces [lift] with applications of [traverse] *)
-  repeat rewrite @expand_unlift;
+  repeat rewrite @expand_lower;
   (* this replaces the generic [traverse] with the user's [_traverse] functions *)
   simpl traverse;
   (* this simplifies applications of each [_traverse] function and folds them back *)
-  repeat simpl_unlift;
+  repeat simpl_lower;
   (* if we have exposed applications of [lift_idx], try simplifying them away *)
-  (* repeat unlift_idx; *)
+  (* repeat lower_idx; *)
   (* if this exposes uses of [var], replace them with the user's [TVar] constructor *)
   simpl var.
 
@@ -1776,4 +1778,5 @@ Qed.
    prevents [simpl] from unfolding the definitions and making a mess. *)
 
 Global Opaque lift.
+Global Opaque lower.
 Global Opaque subst.
